examples/Incubator.thy
@@ -1,6 +1,8 @@
+section \<open> Incubator \<close>
+
 theory Incubator
-  imports "Interaction_Trees.ITree_Simulation" "Interaction_Trees.ITree_Eval"
-    "Z_Toolkit.Z_Toolkit" "../ITree_Machine" "HOL-Library.Code_Target_Int"
+  imports "Interaction_Trees.ITree_Simulation" "Interaction_Trees.ITree_Machine"
+    "Z_Toolkit.Z_Toolkit" "HOL-Library.Code_Target_Int"
 begin
 
 lit_vars
@@ -22,31 +24,40 @@ schema IncubatorMonitor =
 
 record_default IncubatorMonitor
 
+expr_ctr IncubatorMonitor_inv
+expr_ctr IncubatorMonitor
+
 zoperation Increment =
   over IncubatorMonitor
   guard "temp < MAX_TEMP"
   update "[temp \<leadsto> temp + 1]"
 
+lemma Increment_correct: "\<^bold>{IncubatorMonitor\<^bold>} Increment() \<^bold>{IncubatorMonitor\<^bold>}"
+  unfolding Increment_def IncubatorMonitor_inv_def by hoare_wlp
+
 zoperation Decrement =
   over IncubatorMonitor
-  guard "temp > MIN_TEMP"
+  guard "temp > MIN_TEMP" \<comment> \<open> Change to @{term "(temp \<ge> MIN_TEMP)\<^sub>e"} to break the invariant \<close>
   update "[temp \<leadsto> temp - 1]"
+
+lemma Decrement_correct: "\<^bold>{IncubatorMonitor\<^bold>} Decrement() \<^bold>{IncubatorMonitor\<^bold>}"
+  unfolding Decrement_def IncubatorMonitor_inv_def by hoare_wlp
 
 zoperation GetTemp =
   over IncubatorMonitor
   params currentTemp \<in> TEMP
   post "temp = currentTemp"
 
+lemma GetTemp_correct: "\<^bold>{IncubatorMonitor\<^bold>} GetTemp v \<^bold>{IncubatorMonitor\<^bold>}"
+  unfolding GetTemp_def IncubatorMonitor_inv_def by hoare_wlp
+
 zmachine Incubator =
   init "[temp \<leadsto> 20]"
   operations Increment Decrement GetTemp
 
-
 code_datatype pfun_of_alist pfun_of_map
 
-
 simulate Incubator
-
 
 end
   
